prove func_spec_combine lemmas

core/FuncSpec.v
@@ -5,6 +5,10 @@ Require Import Poulet4.Value.
 Require Import Poulet4.Semantics.
 Require Import ProD3.core.Coqlib.
 Require Import ProD3.core.Hoare.
+Require ProD3.core.AssertionLang.
+Require Import ProD3.core.AssertionNotations.
+Require Import ProD3.core.ConcreteHoare.
+Require Import Hammer.Plugin.Hammer.
 
 Section FuncSpec.
 
@@ -22,12 +26,119 @@ Definition hoare_func_modifies (ge : genv) (p : path) (func : @fundef tags_t) (v
   forall st inargs targs st' outargs sig,
     exec_func ge read_ndetbit p st func targs inargs st' outargs sig ->
     (forall q, ~(In q vars) -> PathMap.get q (get_memory st) = PathMap.get q (get_memory st'))
-    /\ (forall q, ~(In q exts) -> PathMap.get q (get_memory st) = PathMap.get q (get_memory st')).
+    /\ (forall q, ~(In q exts) -> PathMap.get q (snd st) = PathMap.get q (snd st')).
 
 Definition hoare_func_spec (ge : genv) (p : path) (pre : arg_assertion)
     (func : @fundef tags_t) (targs : list P4Type) (post : arg_ret_assertion)
     (vars : list path) (exts : list path) :=
   hoare_func ge p pre func targs post
     /\ hoare_func_modifies ge p func vars exts.
+
+Definition path_eq_dec : forall (p p' : path), {p = p'} + {p <> p'}.
+Proof.
+  apply list_eq_dec, String.string_dec.
+Defined.
+
+Definition exclude {A} (mods : list path) (l : list (path * A)) :=
+  filter (fun '(p, _) => negb (In_dec path_eq_dec p mods)) l.
+
+Definition hoare_func_frame (ge : genv) (p : path) (pre : arg_assertion) (func : @fundef tags_t) (targs : list P4Type) (post : assertion) :=
+  forall st inargs st' outargs sig,
+    pre inargs st ->
+    exec_func ge read_ndetbit p st func targs inargs st' outargs sig ->
+    post st'.
+
+Lemma hoare_func_frame_intro : forall ge p a_arg a_mem a_ext func targs vars exts a_mem' a_ext',
+  hoare_func_modifies ge p func vars exts ->
+  exclude vars a_mem = a_mem' ->
+  exclude exts a_ext = a_ext' ->
+  hoare_func_frame ge p (ARG a_arg (MEM a_mem (EXT a_ext))) func targs (MEM a_mem' (EXT a_ext')).
+Proof.
+  unfold hoare_func_modifies, hoare_func_frame; intros.
+  specialize (H _ _  _ _ _ _ H3).
+  destruct H.
+  destruct st; destruct st'.
+  destruct H2 as [_ []].
+  split.
+  - clear -H H0 H2.
+    generalize dependent a_mem'.
+    induction a_mem; intros.
+    + subst. constructor.
+    + simpl in H0. destruct a as [p ?]. destruct (in_dec path_eq_dec p vars) as [H_In | H_In].
+      * subst; simpl. apply IHa_mem; auto.
+        inv H2; auto.
+      * subst; simpl. constructor. 
+        ++simpl in H; simpl.
+          rewrite <- H by auto.
+          inv H2; auto.
+        ++apply IHa_mem; auto.
+          inv H2; auto.
+  - clear -H1 H5 H4.
+    generalize dependent a_ext'.
+    induction a_ext; intros.
+    + subst. constructor.
+    + simpl in H1. destruct a as [p ?]. destruct (in_dec path_eq_dec p exts) as [H_In | H_In].
+      * subst; simpl. apply IHa_ext; auto.
+        inv H5; auto.
+      * subst; simpl. constructor. 
+        ++simpl in H4; simpl.
+          rewrite <- H4 by auto.
+          inv H5; auto.
+        ++apply IHa_ext; auto.
+          inv H5; auto.
+Qed.
+
+Inductive func_post_combine : assertion -> arg_ret_assertion -> arg_ret_assertion -> Prop :=
+  | func_post_combine_base : forall f_mem f_ext a_arg a_ret a_mem a_ext,
+      func_post_combine
+        (MEM f_mem (EXT f_ext))
+        (ARG_RET a_arg a_ret (MEM a_mem (EXT a_ext)))
+        (ARG_RET a_arg a_ret (MEM (f_mem ++ a_mem) (EXT (f_ext ++ a_ext))))
+  | func_post_combine_ex : forall [A] F (P : A -> arg_ret_assertion) Q,
+      (forall (x : A), func_post_combine F (P x) (Q x)) ->
+      func_post_combine F (arg_ret_exists P) (arg_ret_exists Q).
+
+Lemma func_post_combine_sound : forall outargs retv st F P Q,
+  func_post_combine F P Q ->
+  F st ->
+  P outargs retv st ->
+  Q outargs retv st.
+Proof.
+  intros. induction H.
+  - destruct H1 as [? []].
+    split; eauto.
+    split; eauto.
+    destruct st; split.
+    + apply AssertionLang.mem_denote_app. sfirstorder.
+    + apply AssertionLang.ext_denote_app. sfirstorder.
+  - destruct H1.
+    eexists; eauto.
+Qed.
+
+Lemma func_spec_combine : forall ge p pre func targs post vars exts post' frame,
+  hoare_func_spec ge p pre func targs post' vars exts ->
+  hoare_func_frame ge p pre func targs frame ->
+  func_post_combine frame post' post ->
+  hoare_func ge p pre func targs post.
+Proof.
+  unfold hoare_func; intros.
+  destruct H.
+  epose proof (H _ _ _ _ _ ltac:(eassumption) ltac:(eassumption)).
+  destruct sig; only 1, 3, 4 : solve [inv H5].
+  eapply (func_post_combine_sound _ _ _ _ _ _ H1); eauto.
+Qed.
+
+Lemma func_spec_combine' : forall ge p pre_arg pre_mem pre_ext func targs post vars exts post' f_mem f_ext,
+  hoare_func_spec ge p (ARG pre_arg (MEM pre_mem (EXT pre_ext))) func targs post' vars exts ->
+  exclude vars pre_mem = f_mem ->
+  exclude exts pre_ext = f_ext ->
+  func_post_combine (MEM f_mem (EXT f_ext)) post' post ->
+  hoare_func ge p (ARG pre_arg (MEM pre_mem (EXT pre_ext))) func targs post.
+Proof.
+  intros.
+  eapply func_spec_combine; eauto.
+  destruct H.
+  eapply hoare_func_frame_intro; eauto.
+Qed.
 
 End FuncSpec.
